coq/lib/Utils/VecUtil.v
@@ -3,8 +3,12 @@ Module Vec := Coq.Vectors.Vector.
 From Equations Require Import Equations.
 Require Import Poulet4.Utils.Util.FunUtil.
 
+Derive NoConfusion NoConfusionHom Subterm for nat.
+
 Module VecEquations.
-  Derive Signature NoConfusion NoConfusionHom for Vec.t.
+  Derive Signature NoConfusion NoConfusionHom Subterm for Vec.t.
+
+  Derive Signature for Vec.Forall.
 End VecEquations.
 
 Definition vec_sum {n : nat} (v : Vec.t nat n) : nat :=
@@ -17,6 +21,26 @@ Section Lemmas.
   Polymorphic Universe a.
   Polymorphic Context {A : Type@{a}}.
 
+  Section ForallForall.
+    Polymorphic Variable P : A -> Prop.
+
+    Local Hint Constructors Vec.Forall : core.
+    
+    Polymorphic Lemma list_Forall_vec : forall (l : list A),
+        List.Forall P l -> Vec.Forall P (Vec.of_list l).
+    Proof using.
+      intros l h; induction h; cbn; auto.
+    Qed.
+
+    Local Hint Constructors List.Forall : core.
+
+    Polymorphic Lemma vec_Forall_list : forall {n : nat} (v : Vec.t A n),
+        Vec.Forall P v -> List.Forall P (Vec.to_list v).
+    Proof using.
+      intros n v h. depind h; cbn; auto.
+    Qed.
+  End ForallForall.
+  
   Polymorphic Fixpoint vec_rep (n : nat) (a : A) : Vec.t A n :=
     match n with
     | O => []
@@ -26,6 +50,37 @@ Section Lemmas.
   Polymorphic Universes b.
   Polymorphic Context {B : Type@{b}}.
 
+  Section Foralloflistmap.
+    Polymorphic Variable f : A -> B.
+
+    Polymorphic Lemma map_to_list : forall {n} (v : Vec.t A n),
+        List.map f (Vec.to_list v) = Vec.to_list (Vec.map f v).
+    Proof using.
+      intros n v. depind v; cbn; f_equal; auto.
+    Qed.
+    
+    Polymorphic Variable P : B -> Prop.
+
+    Local Hint Constructors Vec.Forall : core.
+    
+    Polymorphic Lemma Forall_of_list_map : forall (l : list A),
+        Vec.Forall P (Vec.of_list (List.map f l)) ->
+        Vec.Forall P (Vec.map f (Vec.of_list l)).
+    Proof using.
+      intro l; induction l as [| a l ih]; intro h; cbn in *; depelim h; auto.
+    Qed.
+
+    Polymorphic Lemma Forall_map_of_list : forall (l : list A),
+        Vec.Forall P (Vec.map f (Vec.of_list l)) ->
+        Vec.Forall P (Vec.of_list (List.map f l)).
+    Proof using.
+      intro l; induction l as [| a l ih]; intro h; cbn in *; depelim h; auto.
+    Qed.
+  End Foralloflistmap.
+  
+  (*Polymorphic Lemma map_of_list : forall (f : A -> B) (l : list A),
+    Vec.of_list (List.map f l) = Vec.map f (Vec.of_list l).*)
+  
   Polymorphic Lemma vec_map2_same : forall {n : nat} (f : A -> A -> B) (v : Vec.t A n),
       Vec.map2 f v v = Vec.map (fun a => f a a) v.
   Proof using.
@@ -39,6 +94,22 @@ Section Lemmas.
       vec_zip (a :: va) (b :: vb) := (a, b) :: vec_zip va vb
     }.
 
+  Polymorphic Lemma vec_zip_fst : forall {n : nat} (va : Vec.t A n) (vb : Vec.t B n),
+      Vec.map fst (vec_zip va vb) = va.
+  Proof using.
+    intros n va vb.
+    funelim (vec_zip va vb); auto.
+    rewrite vec_zip_equation_2; cbn; f_equal; auto.
+  Qed.
+
+  Polymorphic Lemma vec_zip_snd : forall {n : nat} (va : Vec.t A n) (vb : Vec.t B n),
+      Vec.map snd (vec_zip va vb) = vb.
+  Proof using.
+    intros n va vb.
+    funelim (vec_zip va vb); auto.
+    rewrite vec_zip_equation_2; cbn; f_equal; auto.
+  Qed.
+  
   Polymorphic Equations vec_unzip : forall {n : nat},
       Vec.t (A * B) n -> Vec.t A n * Vec.t B n := {
       vec_unzip [] := ([], []);
@@ -46,6 +117,15 @@ Section Lemmas.
         let '(va, vb) := vec_unzip v in (a :: va, b :: vb)
     }.
 
+  Polymorphic Lemma vec_unzip_correct : forall {n : nat} (v : Vec.t (A * B) n),
+      vec_unzip v = (Vec.map fst v, Vec.map snd v).
+  Proof using.
+    intros n v.
+    funelim (vec_unzip v); cbn; auto.
+    rewrite vec_unzip_equation_2, H.
+    reflexivity.
+  Qed.
+  
   Polymorphic Universes c.
   Polymorphic Context {C : Type@{c}}.
   
@@ -101,3 +181,34 @@ Section Lemmas.
     destruct h as [b a]. f_equal. assumption.
   Qed.
 End Lemmas.
+
+Section Map3.
+  Import Vec.VectorNotations.
+  Local Open Scope vector_scope.
+  
+  Polymorphic Universes a b c d.
+  Polymorphic Context {A : Type@{a}} {B : Type@{b}} {C : Type@{c}} {D : Type@{d}}.
+  Polymorphic Variable f : A -> B -> C -> D.
+
+  Set Equations Transparent.
+  
+  Polymorphic Equations vec_map3 :
+    forall {n : nat}, Vec.t A n -> Vec.t B n -> Vec.t C n -> Vec.t D n := {
+      vec_map3 [] [] [] := [];
+      vec_map3 (a :: v1) (b :: v2) (c :: v3) :=
+        f a b c :: vec_map3 v1 v2 v3
+    }.
+End Map3.
+
+Section MapRep.
+  Polymorphic Universes a b.
+  Polymorphic Context {A : Type@{a}} {B : Type@{b}}.
+  Polymorphic Variable f : A -> B.
+  Polymorphic Variable a : A.
+
+  Polymorphic Lemma vec_rep_map : forall n,
+      Vec.map f (vec_rep n a) = vec_rep n (f a).
+  Proof using.
+    intro n; induction n as [| n ih]; cbn; f_equal; assumption.
+  Qed.
+End MapRep.
